Micro_Rust_Parser_Tests/Parser_Test_Expr_Types.thy
@@ -1,0 +1,892 @@
+theory Parser_Test_Expr_Types
+  imports Parser_Test_Utils
+begin
+
+section\<open> Common elaboration API \<close>
+
+ML_val\<open>
+  local
+    val ctxt = \<^context>
+    val source_pos =
+      Position.make0 11 100 0 "" "urust-common-api" ""
+    val argument_pos =
+      Position.make0 13 200 0 "" "urust-common-api" ""
+
+    fun source text =
+      Parser_Lex_Util.positioned_content_source text source_pos
+
+    fun elaborate kind text arguments declared_type =
+      URust_Command.elaborate ctxt
+        {kind = kind,
+         source = source text,
+         arguments = arguments,
+         arguments_pos = argument_pos,
+         declared_type = declared_type}
+
+    val untyped =
+      elaborate URust_Command.Expression
+        "\<llangle>1 :: nat\<rrangle>" [] NONE
+    val typed_expression_type =
+      "(unit, nat, unit, unit, unit, unit) expression"
+    val typed_expression =
+      elaborate URust_Command.Expression
+        "\<llangle>1 :: nat\<rrangle>" []
+        (SOME (typed_expression_type, Position.line 17))
+    val typed_function_type =
+      "nat \<Rightarrow> (unit, nat, unit, unit, unit) function_body"
+    val typed_function =
+      elaborate URust_Command.Function
+        "item" [("item", argument_pos)]
+        (SOME (typed_function_type, Position.line 19))
+
+    fun count_constant expected =
+      Term.fold_aterms
+        (fn Const (actual, _) =>
+              if actual = expected then Integer.add 1 else I
+          | _ => I)
+
+    val _ =
+      (case Term.body_type (fastype_of untyped) of
+         Type (name, _) =>
+           if name = \<^type_name>\<open>expression\<close> then ()
+           else error "common elaborator: untyped expression result changed"
+       | _ => error "common elaborator: untyped expression type disappeared")
+    val _ =
+      if fastype_of typed_expression =
+          Syntax.read_typ ctxt typed_expression_type
+      then ()
+      else error "common elaborator: typed expression constraint was not preserved"
+    val _ =
+      if fastype_of typed_function =
+          Syntax.read_typ ctxt typed_function_type
+      then ()
+      else error "common elaborator: typed function constraint was not preserved"
+    val _ =
+      if count_constant \<^const_name>\<open>FunctionBody\<close>
+          typed_expression 0 = 0
+      then ()
+      else error "common elaborator: expression gained a FunctionBody wrapper"
+    val _ =
+      if count_constant \<^const_name>\<open>FunctionBody\<close>
+          typed_function 0 = 1
+      then ()
+      else error "common elaborator: function wrapper count changed"
+  in
+    val _ = ()
+  end
+\<close>
+
+
+section\<open> Typed declaration surface \<close>
+
+declare [[urust_conformance_check = true]]
+
+urust_expr typed_closed ::
+  \<open>(unit, nat, unit, unit, unit, unit) expression\<close>
+  \<open> \<llangle>42 :: nat\<rrangle> \<close>
+
+urust_expr typed_contextual ::
+  \<open>nat \<Rightarrow> (unit, nat, unit, unit, unit, unit) expression\<close>
+  \<open> item \<close>
+  with_args item
+
+urust_expr typed_heterogeneous ::
+  \<open>nat \<Rightarrow> bool \<Rightarrow>
+    (unit, nat \<times> bool, unit, unit, unit, unit) expression\<close>
+  \<open> \<llangle>(number, flag)\<rrangle> \<close>
+  with_args number flag
+
+urust_expr typed_higher_order ::
+  \<open>(nat \<Rightarrow> nat) \<Rightarrow> nat \<Rightarrow>
+    (unit, nat, unit, unit, unit, unit) expression\<close>
+  \<open> \<llangle>f item\<rrangle> \<close>
+  with_args f item
+
+urust_expr typed_polymorphic ::
+  \<open>'a \<Rightarrow> ('s, 'a, 'r, 'abort, 'i, 'o) expression\<close>
+  \<open> item \<close>
+  with_args item
+
+urust_expr typed_sort_constrained ::
+  \<open>'a::len word \<Rightarrow>
+    ('s, 'a word, 'r, 'abort, 'i, 'o) expression\<close>
+  \<open> item \<close>
+  with_args item
+
+urust_expr typed_placeholders ::
+  \<open>_ \<Rightarrow> (_, _, _, _, _, _) expression\<close>
+  \<open> item \<close>
+  with_args item
+
+text\<open>
+A declaration ending in \<open>function_body\<close> selects function elaboration through the same
+\<open>urust_expr\<close> command and therefore wraps the checked body exactly once.
+\<close>
+
+urust_expr typed_function_common ::
+  \<open>nat \<Rightarrow> (unit, nat, unit, unit, unit) function_body\<close>
+  \<open> item \<close>
+  with_args item
+
+thm typed_closed_conformance
+thm typed_contextual_conformance
+thm typed_heterogeneous_conformance
+thm typed_higher_order_conformance
+thm typed_polymorphic_conformance
+thm typed_sort_constrained_conformance
+thm typed_placeholders_conformance
+thm typed_function_common_conformance
+
+
+section\<open> Definitions, abbreviations, flags, locales, and against \<close>
+
+declare [[urust_conformance_check = false]]
+
+urust_expr
+  [urust_conformance_check = false, urust_verbose = false, urust_abbrev = false]
+  typed_flags_000 ::
+  \<open>(unit, unit, unit, unit, unit, unit) expression\<close>
+  \<open> () \<close>
+
+urust_expr
+  [urust_abbrev = true, urust_conformance_check = false, urust_verbose = false]
+  typed_flags_001 ::
+  \<open>(unit, unit, unit, unit, unit, unit) expression\<close>
+  \<open> () \<close>
+
+urust_expr
+  [urust_verbose = true, urust_abbrev = false, urust_conformance_check = false]
+  typed_flags_010 ::
+  \<open>(unit, unit, unit, unit, unit, unit) expression\<close>
+  \<open> () \<close>
+
+urust_expr
+  [urust_conformance_check = false, urust_abbrev = true, urust_verbose = true]
+  typed_flags_011 ::
+  \<open>(unit, unit, unit, unit, unit, unit) expression\<close>
+  \<open> () \<close>
+
+urust_expr
+  [urust_verbose = false, urust_conformance_check = true, urust_abbrev = false]
+  typed_flags_100 ::
+  \<open>(unit, unit, unit, unit, unit, unit) expression\<close>
+  \<open> () \<close>
+
+urust_expr
+  [urust_abbrev = true, urust_verbose = false, urust_conformance_check = true]
+  typed_flags_101 ::
+  \<open>(unit, unit, unit, unit, unit, unit) expression\<close>
+  \<open> () \<close>
+
+urust_expr
+  [urust_conformance_check = true, urust_verbose = true, urust_abbrev = false]
+  typed_flags_110 ::
+  \<open>(unit, unit, unit, unit, unit, unit) expression\<close>
+  \<open> () \<close>
+
+urust_expr
+  [urust_verbose = true, urust_abbrev = true, urust_conformance_check = true]
+  typed_flags_111 ::
+  \<open>(unit, unit, unit, unit, unit, unit) expression\<close>
+  \<open> () \<close>
+
+urust_expr
+  [urust_abbrev = true, urust_conformance_check = true, urust_verbose = true]
+  typed_function_abbrev_common ::
+  \<open>nat \<Rightarrow> (unit, nat, unit, unit, unit) function_body\<close>
+  \<open> item \<close>
+  with_args item
+
+urust_expr typed_against ::
+  \<open>32 word \<Rightarrow>
+    (unit, 32 word, unit, unit, unit, unit) expression\<close>
+  \<open> operand + 1u32 \<close>
+  with_args operand
+  against \<open> \<lbrakk> operand + 1_u32 \<rbrakk> \<close>
+
+locale typed_expression_locale =
+  fixes offset :: nat
+begin
+
+urust_expr
+  [urust_abbrev = true, urust_conformance_check = true]
+  typed_local_add ::
+  \<open>nat \<Rightarrow> (unit, nat, unit, unit, unit, unit) expression\<close>
+  \<open> \<llangle>item + offset\<rrangle> \<close>
+  with_args item
+
+end
+
+definition typed_flags_abbrev_client where
+  \<open>typed_flags_abbrev_client = typed_flags_001\<close>
+
+ML_val\<open>
+  local
+    val ctxt = \<^context>
+    val thy = Proof_Context.theory_of ctxt
+    val consts = Proof_Context.consts_of ctxt
+
+    fun assert message condition =
+      if condition then ()
+      else error ("typed declaration artifact audit: " ^ message)
+
+    fun has_fact name = can (Proof_Context.get_thm ctxt) name
+
+    fun constant_name name = Consts.intern consts name
+
+    fun is_abbreviation name =
+      can (Consts.the_abbreviation consts) (constant_name name)
+
+    fun executable_equations name =
+      (case Exn.result (Code.get_cert ctxt []) (constant_name name) of
+         Exn.Res certificate =>
+           let
+             val (_, equations) =
+               Code.equations_of_cert thy certificate
+           in
+             map_filter
+               (fn (_, (SOME theorem, _)) => SOME theorem
+                 | _ => NONE)
+               (the equations)
+           end
+       | Exn.Exn exn =>
+           if Exn.is_interrupt exn then Exn.reraise exn else [])
+
+    val definitions =
+      ["typed_closed", "typed_contextual", "typed_heterogeneous",
+       "typed_higher_order", "typed_polymorphic",
+       "typed_sort_constrained", "typed_placeholders",
+       "typed_function_common", "typed_flags_000", "typed_flags_010",
+       "typed_flags_100", "typed_flags_110", "typed_against"]
+    val abbreviations =
+      ["typed_flags_001", "typed_flags_011",
+       "typed_flags_101", "typed_flags_111",
+       "typed_function_abbrev_common"]
+    val conforming =
+      ["typed_closed", "typed_contextual", "typed_heterogeneous",
+       "typed_higher_order", "typed_polymorphic",
+       "typed_sort_constrained", "typed_placeholders",
+       "typed_function_common", "typed_flags_100",
+       "typed_flags_101", "typed_flags_110", "typed_flags_111",
+       "typed_function_abbrev_common", "typed_against"]
+    val nonconforming =
+      ["typed_flags_000", "typed_flags_001",
+       "typed_flags_010", "typed_flags_011"]
+
+    fun check_definition name =
+      (assert (quote name ^ " is missing its _def fact")
+         (has_fact (name ^ "_def"));
+       assert (quote name ^ " was installed as an abbreviation")
+         (not (is_abbreviation name));
+       assert (quote name ^ " does not have one code equation")
+         (length (executable_equations name) = 1))
+
+    fun check_abbreviation name =
+      (assert (quote name ^ " unexpectedly has a _def fact")
+         (not (has_fact (name ^ "_def")));
+       assert (quote name ^ " was not installed as an abbreviation")
+         (is_abbreviation name);
+       assert (quote name ^ " unexpectedly has a code equation")
+         (null (executable_equations name)))
+
+    val _ = List.app check_definition definitions
+    val _ = List.app check_abbreviation abbreviations
+    val _ =
+      List.app
+        (fn name =>
+          assert (quote name ^ " is missing _conformance")
+            (has_fact (name ^ "_conformance")))
+        conforming
+    val _ =
+      List.app
+        (fn name =>
+          assert (quote name ^ " unexpectedly has _conformance")
+            (not (has_fact (name ^ "_conformance"))))
+        nonconforming
+
+    val abbreviation_proposition =
+      Thm.prop_of
+        (Proof_Context.get_thm ctxt "typed_flags_abbrev_client_def")
+    val abbreviation_name = constant_name "typed_flags_001"
+    val _ =
+      assert "abbreviation survived in a checked client term"
+        (not
+          (Term.exists_subterm
+            (fn Const (name, _) => name = abbreviation_name
+              | _ => false)
+            abbreviation_proposition))
+  in
+    val _ = ()
+  end
+\<close>
+
+
+section\<open> Exact expression and function shape \<close>
+
+ML_val\<open>
+  local
+    val ctxt = \<^context>
+
+    fun definition_rhs name =
+      Proof_Context.get_thm ctxt (name ^ "_def")
+      |> Thm.prop_of
+      |> Logic.dest_equals
+      |> #2
+
+    val expression = definition_rhs "typed_heterogeneous"
+    val function = definition_rhs "typed_function_common"
+    val expression_type =
+      "nat \<Rightarrow> bool \<Rightarrow> " ^
+      "(unit, nat \<times> bool, unit, unit, unit, unit) expression"
+    val function_type =
+      "nat \<Rightarrow> (unit, nat, unit, unit, unit) function_body"
+    val expected_expression =
+      Syntax.check_term ctxt
+        (Type.constraint (Syntax.read_typ ctxt expression_type)
+          (Syntax.parse_term ctxt
+            "(\<lambda>(number :: nat) (flag :: bool). \<lbrakk> \<llangle>(number, flag)\<rrangle> \<rbrakk>)"))
+    val expected_function =
+      Syntax.check_term ctxt
+        (Type.constraint (Syntax.read_typ ctxt function_type)
+          (Syntax.parse_term ctxt
+            "(\<lambda>(item :: nat). FunctionBody \<lbrakk> item \<rbrakk>)"))
+
+    fun count_constant expected =
+      Term.fold_aterms
+        (fn Const (actual, _) =>
+              if actual = expected then Integer.add 1 else I
+          | _ => I)
+
+    val _ =
+      if Term.aconv (expression, expected_expression) then ()
+      else error "typed urust_expr: expression lambda shape changed"
+    val _ =
+      if Term.aconv (function, expected_function) then ()
+      else error "typed urust_expr: function lambda shape changed"
+    val _ =
+      if count_constant \<^const_name>\<open>FunctionBody\<close>
+          expression 0 = 0
+      then ()
+      else error "typed urust_expr: expression gained a FunctionBody wrapper"
+    val _ =
+      if count_constant \<^const_name>\<open>FunctionBody\<close>
+          function 0 = 1
+      then ()
+      else error "typed urust_expr: function wrapper count changed"
+  in
+    val _ = ()
+  end
+\<close>
+
+
+section\<open> Migration-sensitive typed expressions \<close>
+
+declare [[urust_conformance_check = true]]
+
+urust_expr typed_boolean_negation ::
+  \<open>bool \<Rightarrow> ('s, bool, 'r, 'abort, 'i, 'o) expression\<close>
+  \<open> !value \<close>
+  with_args value
+
+urust_expr typed_word_negation ::
+  \<open>'a::len word \<Rightarrow>
+    ('s, 'a word, 'r, 'abort, 'i, 'o) expression\<close>
+  \<open> !value \<close>
+  with_args value
+
+urust_expr typed_bound_negation ::
+  \<open>('s, bool, 'r, 'abort, 'i, 'o) expression \<Rightarrow>
+    ('s, bool, 'r, 'abort, 'i, 'o) expression\<close>
+  \<open> let value = \<epsilon>\<open>source\<close>; !value \<close>
+  with_args source
+
+urust_expr typed_indexing ::
+  \<open>nat list \<Rightarrow> 64 word \<Rightarrow>
+    ('s, nat, 'r, 'abort, 'i, 'o) expression\<close>
+  \<open> values[index] \<close>
+  with_args values index
+
+urust_expr typed_abort_sequence ::
+  \<open>'abort abort \<Rightarrow>
+    ('s, 'v, 'r, 'abort, 'i, 'o) expression \<Rightarrow>
+    ('s, 'v, 'r, 'abort, 'i, 'o) expression\<close>
+  \<open> \<epsilon>\<open>abort reason\<close>; \<epsilon>\<open>tail\<close> \<close>
+  with_args reason tail
+
+urust_expr typed_panic_sequence ::
+  \<open>String.literal \<Rightarrow>
+    ('s, 'v, 'r, 'abort, 'i, 'o) expression \<Rightarrow>
+    ('s, 'v, 'r, 'abort, 'i, 'o) expression\<close>
+  \<open> panic!(message); \<epsilon>\<open>tail\<close> \<close>
+  with_args message tail
+
+definition typed_channel_get :: \<open>nat \<Rightarrow> nat option\<close>
+  where \<open>typed_channel_get state = Some state\<close>
+
+definition typed_channel_put :: \<open>nat \<Rightarrow> nat \<Rightarrow> nat\<close>
+  where \<open>typed_channel_put value state = value + state\<close>
+
+urust_expr typed_channel_inference ::
+  \<open>(nat, unit, unit, 'abort, 'i, 'o) expression\<close>
+  \<open>
+    if let Some(value) = \<epsilon>\<open>get typed_channel_get\<close> {
+      \<epsilon>\<open>put (typed_channel_put value)\<close>
+    }
+  \<close>
+
+urust_expr typed_captured_nil ::
+  \<open>
+    (nat \<Rightarrow> nat) \<Rightarrow>
+    (nat \<Rightarrow> bool) \<Rightarrow>
+    tnil \<Rightarrow>
+    (nat \<Rightarrow> bool \<Rightarrow>
+      (nat, nat \<times> bool, unit, unit, unit, unit) expression) \<Rightarrow>
+    (nat, nat \<times> bool, unit, unit, unit, unit) expression
+  \<close>
+  \<open>
+    let (left, right) =
+      \<epsilon>\<open>get (\<lambda>state. (f state, g state, nil))\<close>;
+    \<epsilon>\<open>continuation left right\<close>
+  \<close>
+  with_args f g nil continuation
+
+thm typed_boolean_negation_conformance
+thm typed_word_negation_conformance
+thm typed_bound_negation_conformance
+thm typed_indexing_conformance
+thm typed_abort_sequence_conformance
+thm typed_panic_sequence_conformance
+thm typed_channel_inference_conformance
+thm typed_captured_nil_conformance
+
+
+section\<open> Rejections, positions, and recovery \<close>
+
+ML_val\<open>
+  local
+    val ctxt = \<^context>
+    val file = "urust-typed-api-rejection"
+    val type_pos = Position.make0 3 30 0 "" file ""
+    val arguments_pos = Position.make0 5 50 0 "" file ""
+    val source_pos = Position.make0 7 70 0 "" file ""
+
+    fun fail message =
+      error ("typed elaboration rejection audit: " ^ message)
+
+    fun source text =
+      Parser_Lex_Util.positioned_content_source text source_pos
+
+    fun argument line offset name =
+      (name, Position.make0 line offset 0 "" file "")
+
+    fun elaborate kind raw_type arguments body =
+      URust_Command.elaborate ctxt
+        {kind = kind,
+         source = source body,
+         arguments = arguments,
+         arguments_pos = arguments_pos,
+         declared_type = Option.map (fn typ => (typ, type_pos)) raw_type}
+
+    fun rejection_message label action =
+      (case Exn.result action () of
+         Exn.Res term =>
+           fail
+             (label ^ " unexpectedly elaborated as " ^
+               Syntax.string_of_term ctxt term)
+       | Exn.Exn exn =>
+           if Exn.is_interrupt exn then Exn.reraise exn
+           else Runtime.exn_message exn)
+
+    fun expect_rejection label expected action =
+      let val message = rejection_message label action in
+        if String.isSubstring expected message then ()
+        else
+          fail
+            (label ^ " reported " ^ quote message ^
+              " instead of containing " ^ quote expected)
+      end
+
+    fun expect_positioned_rejection label expected lines action =
+      let
+        val message = rejection_message label action
+        val has_expected = String.isSubstring expected message
+        val has_file = String.isSubstring file message
+        val has_lines =
+          forall
+            (fn line =>
+              String.isSubstring ("line " ^ string_of_int line) message)
+            lines
+      in
+        if has_expected andalso has_file andalso has_lines then ()
+        else fail (label ^ " lost its expected position: " ^ quote message)
+      end
+
+    val expression_type =
+      "(unit, nat, unit, unit, unit, unit) expression"
+    val unary_expression_type =
+      "nat \<Rightarrow> " ^ expression_type
+    val binary_expression_type =
+      "nat \<Rightarrow> bool \<Rightarrow> " ^ expression_type
+    val function_type =
+      "nat \<Rightarrow> (unit, nat, unit, unit, unit) function_body"
+
+    val _ =
+      expect_positioned_rejection
+        "missing function type" "requires a declared type" [7]
+        (fn () =>
+          elaborate URust_Command.Function NONE [] "()")
+    val _ =
+      expect_positioned_rejection
+        "wrong function terminal" "result type must be function_body" [3]
+        (fn () =>
+          elaborate URust_Command.Function
+            (SOME unary_expression_type)
+            [argument 11 110 "item"] "item")
+    val _ =
+      expect_positioned_rejection
+        "too few expression arguments" "expects 2 arguments" [5]
+        (fn () =>
+          elaborate URust_Command.Expression
+            (SOME binary_expression_type)
+            [argument 13 130 "number"] "number")
+    val _ =
+      expect_positioned_rejection
+        "too many expression arguments" "expects 1 argument" [17]
+        (fn () =>
+          elaborate URust_Command.Expression
+            (SOME unary_expression_type)
+            [argument 15 150 "item", argument 17 170 "extra"] "item")
+    val _ =
+      expect_rejection
+        "function argument count" "expects 1 parameter"
+        (fn () =>
+          elaborate URust_Command.Function
+            (SOME function_type) [] "0")
+    val _ =
+      expect_positioned_rejection
+        "duplicate typed arguments" "duplicate argument" [19, 23]
+        (fn () =>
+          elaborate URust_Command.Expression
+            (SOME binary_expression_type)
+            [argument 19 190 "same", argument 23 230 "same"] "same")
+    val _ =
+      expect_positioned_rejection
+        "wildcard typed argument" "name `_` is not allowed" [29]
+        (fn () =>
+          elaborate URust_Command.Expression
+            (SOME unary_expression_type)
+            [argument 29 290 "_"] "0")
+    val _ =
+      expect_rejection
+        "argument type mismatch" "Clash of types"
+        (fn () =>
+          elaborate URust_Command.Expression
+            (SOME unary_expression_type)
+            [argument 31 310 "item"] "item == true")
+    val _ =
+      expect_rejection
+        "result type mismatch" "Clash of types"
+        (fn () =>
+          elaborate URust_Command.Expression
+            (SOME "(unit, bool, unit, unit, unit, unit) expression")
+            [] "\<llangle>1 :: nat\<rrangle>")
+    val _ =
+      expect_positioned_rejection
+        "malformed declaration type" "syntax" [3]
+        (fn () =>
+          elaborate URust_Command.Expression
+            (SOME "nat \<Rightarrow>") [] "()")
+
+    val recovered =
+      elaborate URust_Command.Expression
+        (SOME unary_expression_type)
+        [argument 37 370 "item"] "item"
+    val _ =
+      if fastype_of recovered =
+          Syntax.read_typ ctxt unary_expression_type
+      then ()
+      else fail "successful elaboration did not recover after failures"
+  in
+    val _ = ()
+  end
+\<close>
+
+ML_val\<open>
+  local
+    val unit_source = Symbol.open_ ^ " () " ^ Symbol.close
+    val unit_expression_type =
+      Symbol.open_ ^
+      "(unit, unit, unit, unit, unit, unit) expression" ^
+      Symbol.close
+    val unary_expression_type =
+      Symbol.open_ ^
+      "nat \<Rightarrow> (unit, nat, unit, unit, unit, unit) expression" ^
+      Symbol.close
+    val serial = Unsynchronized.ref 0
+
+    fun run_command source_name command_text () =
+      let
+        val thy = \<^theory>
+        val transitions =
+          Outer_Syntax.parse_text thy (K thy)
+            (Position.line_file 1 source_name) command_text
+        val _ =
+          if length transitions = 1 then ()
+          else error "typed command audit: expected exactly one transition"
+      in
+        fold (Toplevel.command_exception false) transitions
+          (Toplevel.make_state (SOME thy))
+      end
+
+    fun recover () =
+      let
+        val index = !serial
+        val _ = serial := index + 1
+      in
+        ignore
+          (run_command ("typed-command-recovery-" ^ string_of_int index)
+            ("urust_expr typed_command_recovered_" ^
+              string_of_int index ^ " :: " ^ unit_expression_type ^
+              " " ^ unit_source) ())
+      end
+
+    fun assert_rejected source_name command_text =
+      (case Exn.result (run_command source_name command_text) () of
+         Exn.Res _ =>
+           error
+             ("typed command was unexpectedly accepted" ^
+               Position.here (Position.file source_name))
+       | Exn.Exn exn =>
+           if Exn.is_interrupt exn then Exn.reraise exn
+           else
+             let
+               val message = Runtime.exn_message exn
+               val _ =
+                 if String.isSubstring source_name message then ()
+                 else
+                   error
+                     ("typed command diagnostic lost its source position:\n" ^
+                       message)
+             in recover () end)
+
+    val _ =
+      assert_rejected "typed-malformed-type"
+        ("urust_expr typed_bad_type :: " ^
+          Symbol.open_ ^ "nat \<Rightarrow>" ^ Symbol.close ^
+          " " ^ unit_source)
+    val _ =
+      assert_rejected "typed-misplaced-type"
+        ("urust_expr typed_misplaced_type " ^ unit_source ^
+          " :: " ^ unit_expression_type)
+    val _ =
+      assert_rejected "typed-duplicate-arguments"
+        ("urust_expr typed_duplicate_arguments :: " ^
+          Symbol.open_ ^
+          "nat \<Rightarrow> nat \<Rightarrow> " ^
+          "(unit, nat, unit, unit, unit, unit) expression" ^
+          Symbol.close ^ " " ^ unit_source ^
+          " with_args item item")
+    val _ =
+      assert_rejected "typed-wildcard-argument"
+        ("urust_expr typed_wildcard_argument :: " ^
+          unary_expression_type ^ " " ^ unit_source ^
+          " with_args _")
+    val _ =
+      assert_rejected "typed-missing-argument"
+        ("urust_expr typed_missing_argument :: " ^
+          unary_expression_type ^ " " ^ unit_source)
+  in
+    val _ = ()
+  end
+\<close>
+
+
+section\<open> Typed binder markup and entity identity \<close>
+
+ML_val\<open>
+  local
+    val ctxt = \<^context>
+    val file = "urust-typed-binder-markup"
+    val document_id = "urust-typed-binder-markup"
+    val first_definition =
+      Position.make0 11 100 0 "" file document_id
+    val second_definition =
+      Position.make0 11 110 0 "" file document_id
+    val body_text =
+      "\<llangle>(first, second, first)\<rrangle>"
+    val body_start =
+      Position.make0 13 200 0 "" file document_id
+    val body_source =
+      Parser_Lex_Util.positioned_content_source body_text body_start
+    val captured =
+      Synchronized.var "urust_typed_binder_markup" ([]: string list)
+    fun capture_reports chunks =
+      Synchronized.change captured (append chunks)
+
+    val _ =
+      Parser_Test_Report_Lock.run (fn () =>
+        Unsynchronized.setmp Private_Output.report_fn capture_reports
+          (fn () =>
+            Print_Mode.with_modes [Print_Mode.PIDE]
+              (fn () =>
+                URust_Command.elaborate ctxt
+                  {kind = URust_Command.Expression,
+                   source = body_source,
+                   arguments =
+                     [("first", first_definition),
+                      ("second", second_definition)],
+                   arguments_pos = Position.line_file 9 file,
+                   declared_type =
+                     SOME
+                       ("nat \<Rightarrow> bool \<Rightarrow> " ^
+                        "(unit, nat \<times> bool \<times> nat, " ^
+                        "unit, unit, unit, unit) expression",
+                        Position.line_file 7 file)}) ())
+          ())
+
+    fun collect (XML.Text _) result = result
+      | collect (XML.Elem (markup, body)) result =
+          fold collect body (markup :: result)
+    val markup =
+      fold collect
+        (maps YXML.parse_body (Synchronized.value captured)) []
+
+    fun find_from needle offset =
+      if offset + size needle > size body_text then
+        error ("typed binder markup audit: missing " ^ quote needle)
+      else if String.substring (body_text, offset, size needle) = needle then
+        offset
+      else find_from needle (offset + 1)
+
+    fun token_position needle offset =
+      let
+        val raw = find_from needle offset
+        val start =
+          Position.symbol_explode
+            (String.substring (body_text, 0, raw)) body_start
+      in
+        (raw,
+         Position.range_position
+           (Position.range (start, Position.symbol_explode needle start)))
+      end
+
+    fun has_position properties position =
+      Properties.get properties Markup.offsetN =
+        Option.map Value.print_int (Position.offset_of position) andalso
+      Properties.get properties Markup.end_offsetN =
+        Option.map Value.print_int (Position.end_offset_of position)
+
+    fun has_markup markup_name position =
+      exists
+        (fn (name, properties) =>
+          name = markup_name andalso has_position properties position)
+        markup
+
+    fun entity_id property position =
+      let
+        val ids =
+          markup
+          |> map_filter
+              (fn (name, properties) =>
+                if name = Markup.entityN andalso
+                   Properties.get properties Markup.kindN =
+                     SOME "urust_var" andalso
+                   has_position properties position
+                then Properties.get properties property
+                else NONE)
+          |> distinct (op =)
+      in
+        (case ids of
+           [id] => id
+         | _ =>
+             error
+               ("typed binder markup audit: entity markup changed at" ^
+                 Position.here position))
+      end
+
+    val (first_offset, first_reference_one) =
+      token_position "first" 0
+    val (second_offset, second_reference) =
+      token_position "second" (first_offset + size "first")
+    val (_, first_reference_two) =
+      token_position "first" (second_offset + size "second")
+    val first_id = entity_id Markup.defN first_definition
+    val second_id = entity_id Markup.defN second_definition
+    val _ =
+      if has_markup Markup.typingN first_definition andalso
+         has_markup Markup.typingN second_definition
+      then ()
+      else error "typed binder markup audit: typed definitions lost tooltips"
+    val _ =
+      if first_id <> second_id then ()
+      else error "typed binder markup audit: arguments reused an entity ID"
+    val _ =
+      if entity_id Markup.refN first_reference_one = first_id andalso
+         entity_id Markup.refN first_reference_two = first_id
+      then ()
+      else error "typed binder markup audit: first references lost navigation"
+    val _ =
+      if entity_id Markup.refN second_reference = second_id then ()
+      else error "typed binder markup audit: second reference lost navigation"
+  in
+    val _ = ()
+  end
+\<close>
+
+
+section\<open> Public facade audit \<close>
+
+ML_val\<open>
+  local
+    val implementation_path =
+      Resources.master_directory \<^theory> +
+        Path.explode "../Micro_Rust_Parser_Impl/Parser_Impl_Command.thy"
+    val implementation = File.read implementation_path
+    val structure_marker =
+      "structure URust_Command :> URUST_COMMAND ="
+    val before_structure =
+      (case first_field structure_marker implementation of
+         SOME (prefix, suffix) =>
+           if is_some (first_field structure_marker suffix)
+           then error "uRust facade audit: command structure is duplicated"
+           else prefix
+       | NONE => error "uRust facade audit: command structure is missing")
+    val signature_marker = "signature URUST_COMMAND ="
+    val signature_text =
+      (case first_field signature_marker before_structure of
+         SOME (_, signature) =>
+           if is_some (first_field signature_marker signature)
+           then error "uRust facade audit: command signature is duplicated"
+           else signature
+       | NONE => error "uRust facade audit: command signature is missing")
+    val exported_values =
+      split_lines signature_text
+      |> filter (String.isPrefix "  val ")
+
+    val _ =
+      if exported_values = ["  val elaborate:"] then ()
+      else
+        error
+          ("uRust facade audit: exported value list changed: " ^
+            commas_quote exported_values)
+    val _ =
+      if String.isSubstring
+          "datatype elaboration_kind = Expression | Function"
+          signature_text
+      then ()
+      else error "uRust facade audit: elaboration_kind is not exported"
+    val _ =
+      List.app
+        (fn removed =>
+          if String.isSubstring removed implementation then
+            error
+              ("uRust facade audit: compatibility alias remains: " ^
+                quote removed)
+          else ())
+        ["elab_urust", "elab_urust_with_args", "elab_urust_fun"]
+  in
+    val _ = ()
+  end
+\<close>
+
+end
